order-book/verify/Properties/OrderV2.lean
@@ -1,0 +1,19 @@
+import Blaster
+import Properties.Soundness
+
+namespace Properties.OrderV2
+
+open PlutusCore.UPLC.Term (Program)
+open Properties.Soundness (spend_sound_theorem)
+
+set_option warn.sorry false
+
+#import_uplc orderV2Script PlutusV3 flat_hex "Scripts/order_v2_spend.flat"
+
+def orderV2Validator : Program := orderV2Script.script
+
+theorem spend_sound :
+  spend_sound_theorem orderV2Validator
+  := by blaster
+
+end Properties.OrderV2
